\documentclass[12pt,english]{article}
\usepackage{lmodern}
\linespread{1.05}
%\usepackage{mathpazo}
%\usepackage{mathptmx}
%\usepackage{utopia}
\usepackage{microtype}
\usepackage{placeins}
\usepackage[T1]{fontenc}
\usepackage[latin9]{inputenc}
\usepackage[dvipsnames]{xcolor}
\usepackage{geometry}
\usepackage{amsthm}
\usepackage{amsfonts}
\usepackage{svg}
\usepackage{booktabs}
\usepackage{caption}
\usepackage{blindtext}
%\renewcommand{\arraystretch}{1.2}
\usepackage{multirow}
\usepackage{float}

% TikZ stuff

\usepackage{tikz}
\usepackage{mathdots}
\usepackage{yhmath}
\usepackage{cancel}
\usepackage{color}
\usepackage{siunitx}
\usepackage{array}
\usepackage{amssymb}
\usepackage{gensymb}
\usepackage{tabularx}
\usetikzlibrary{fadings}
\usetikzlibrary{patterns}
\usetikzlibrary{shadows.blur}






%\usepackage{caption}
%\captionsetup{justification=raggedright,singlelinecheck=false}

\usepackage{courier}
\usepackage{verbatim}
\usepackage[round]{natbib}
\bibliographystyle{plainnat}

\definecolor{red1}{RGB}{128,0,0}
%\geometry{verbose,tmargin=1.25in,bmargin=1.25in,lmargin=1.25in,rmargin=1.25in}
\geometry{verbose,tmargin=1in,bmargin=1in,lmargin=1in,rmargin=1in}
\usepackage{setspace}

\usepackage[colorlinks=true, linkcolor={red!70!black}, citecolor={blue!50!black}, urlcolor={blue!80!black}]{hyperref}
%\usepackage{esint}
\onehalfspacing
\usepackage{babel}
\usepackage{amsmath}
\usepackage{graphicx}

\theoremstyle{remark}
\newtheorem{remark}{Remark}
\begin{document}
	
\title{No exponent on $q_j$}
\author{Nicolas Fernandez-Arias}
\maketitle

Have

\begin{align*}
Y = F(L,\{q_j\},\{k_j\}) &= \frac{L^{\beta}}{1-\beta} \int_0^1 (q_j k_j)^{1-\beta} dj
\end{align*}

And
\begin{align*}
k_j = H(l_j,q_j,Q)
\end{align*}

What assumption on $H$ to get BGP, and what are its properties?

Well, demand curve given prices $p_j$ is defined by 
\begin{align*}
	\max_{k_j} \int_0^1 (q_j k_j)^{1-\beta} dj 
\end{align*}
subject to 
\begin{align*}
	\int_0^1 p_j k_j dj \le E
\end{align*}

Lagrangean:
\begin{align*}
	\mathcal{L} &= \int_0^1 (q_j k_j)^{1-\beta} dj  + \lambda \big(E -\int_0^1 p_j k_j dj  \big)
\end{align*}

FOC:
\begin{align*}
	(1-\beta) q_j^{1-\beta} k_j^{-\beta} &= \lambda p_j \\
	(1-\beta) q_j^{1-\beta} k_j^{1-\beta} &= \lambda k_j p_j
\end{align*}

Dividing the FOC for $j'$ by the FOC for $j$ get
\begin{align*}
	\Big (\frac{q_j k_j}{q_{j'} k_{j'}} \Big)^{1-\beta} &= \frac{p_j k_j}{p_{j'} k_{j'}}
\end{align*}

so 
\begin{align*}
	E &= \int_0^1 p_j k_j dj \\
	  &= \int_0^1 \Big (\frac{q_j k_j}{q_{j'} k_{j'}} \Big)^{1-\beta} p_{j'} k_{j'} dj \\
	  &= \frac{p_{j'} k_{j'}}{\big(q_{j'} k_{j'}\big)^{1-\beta}} \int_0^1 \big( {q_j} {k_j} \big)^{1-\beta}  dj \\
	  &= \frac{p_{j'}}{q_{j'}^{1-\beta}} k_{j'}^{\beta} K \\
	\frac{E}{K p_{j'}} &= \frac{k_{j'}^{\beta}}{q_{j'}^{1-\beta}} 
\end{align*}








\end{document}